template-coq/theories/utils/ReflectEq.v
@@ -1,0 +1,159 @@
+From Coq Require Import ssreflect ssrbool List.
+From Equations Require Import Equations.
+Import ListNotations.
+
+(* Some reflection / EqDec lemmata *)
+
+Class ReflectEq A := {
+  eqb : A -> A -> bool ;
+  eqb_spec : forall x y : A, reflect (x = y) (eqb x y)
+}.
+Arguments eqb : simpl never.
+Infix "==" := eqb (at level 20).
+
+Lemma eqb_eq {A} `{ReflectEq A} (x y : A) : x == y -> x = y.
+Proof.
+  elim: eqb_spec; auto.
+  discriminate.
+Qed.
+
+Lemma eqb_refl {A} {R : ReflectEq A} (x : A) : x == x.
+Proof.
+  destruct (eqb_spec x x); auto.
+Qed.
+
+Lemma neqb {A} {R : ReflectEq A} (x y : A) : ~~ x == y <-> x <> y.
+Proof.
+  destruct (eqb_spec x y); auto; subst; intuition auto.
+Qed.
+
+#[global] Instance ReflectEq_EqDec :
+  forall A, ReflectEq A -> EqDec A.
+Proof.
+  intros A [eqb h] x y.
+  destruct (h x y).
+  - left. assumption.
+  - right. assumption.
+Defined.
+
+Definition eq_dec_to_bool {A} `{EqDec A} x y :=
+  match eq_dec x y with
+  | left _ => true
+  | right _ => false
+  end.
+
+(* Not an instance to avoid loops and making boolean definitions depend on sumbool ones *)
+#[global]
+Lemma EqDec_ReflectEq : forall A `{EqDec A}, ReflectEq A.
+Proof.
+  intros A h.
+  unshelve econstructor.
+  - eapply eq_dec_to_bool.
+  - unfold eq_dec_to_bool.
+    intros x y. destruct (eq_dec x y).
+    all: constructor ; assumption.
+Defined.
+
+Ltac nodec :=
+  let bot := fresh "bot" in
+  try solve [ constructor ; intro bot ; inversion bot ; subst ; tauto ].
+
+Definition eq_option {A} (eqA : A -> A -> bool) (u v : option A) : bool :=
+  match u, v with
+  | Some u, Some v => eqA u v
+  | None, None => true
+  | _, _ => false
+  end.
+
+#[global] Instance reflect_option : forall {A}, ReflectEq A -> ReflectEq (option A).
+Proof.
+  intros A RA. refine {| eqb := eq_option eqb |}.
+  intros x y. destruct x, y.
+  all: cbn.
+  all: try solve [ constructor ; easy ].
+  destruct (eqb_spec a a0) ; nodec.
+  constructor. f_equal. assumption.
+Defined.
+
+Fixpoint eq_list {A} (eqA : A -> A -> bool) (l l' : list A) : bool :=
+  match l, l' with
+  | a :: l, a' :: l' =>
+    if eqA a a' then eq_list eqA l l'
+    else false
+  | [], [] => true
+  | _, _ => false
+  end.
+
+#[global] Instance reflect_list : forall {A}, ReflectEq A -> ReflectEq (list A).
+Proof.
+  intros A RA. refine {| eqb := eq_list eqb |}.
+  intro x. induction x ; intro y ; destruct y.
+  - cbn. constructor. reflexivity.
+  - cbn. constructor. discriminate.
+  - cbn. constructor. discriminate.
+  - cbn. destruct (eqb_spec a a0) ; nodec.
+    destruct (IHx y) ; nodec.
+    subst. constructor. reflexivity.
+Defined.
+
+#[global] Instance reflect_nat : ReflectEq nat := {
+  eqb_spec := PeanoNat.Nat.eqb_spec
+}.
+
+
+Definition eq_bool b1 b2 : bool :=
+  if b1 then b2 else negb b2.
+
+Local Obligation Tactic := idtac.
+
+#[global, program] Instance reflect_bool : ReflectEq bool := {
+  eqb := eq_bool
+}.
+Next Obligation.
+  intros x y. unfold eq_bool.
+  destruct x, y.
+  all: constructor.
+  all: try reflexivity.
+  all: discriminate.
+Defined.
+
+Definition eq_sig_true {A f} `{ReflectEq A} (x y : { z : A | f z = true }) : bool :=
+  proj1_sig x == proj1_sig y.
+
+#[global, program] Instance reflect_sig_true {A f} `{ReflectEq A} : ReflectEq ({ z : A | f z = true }) := {
+  eqb := eq_sig_true
+}.
+Next Obligation.
+  intros A f RA. intros [x hx] [y hy]. unfold eq_sig_true; cbn.
+  destruct (eqb_spec x y) ; nodec. subst.
+  constructor. pose proof (uip hx hy). subst. reflexivity.
+Defined.
+
+
+Definition eq_prod {A B} (eqA : A -> A -> bool) (eqB : B -> B -> bool) x y :=
+  let '(a1, b1) := x in
+  let '(a2, b2) := y in
+  if eqA a1 a2 then eqB b1 b2
+  else false.
+
+#[global, program] Instance reflect_prod : forall {A B}, ReflectEq A -> ReflectEq B -> ReflectEq (A * B) := {
+  eqb := eq_prod eqb eqb
+}.
+Next Obligation.
+  intros A B RA RB [x y] [u v].
+  unfold eq_prod.
+  destruct (eqb_spec x u) ; nodec.
+  destruct (eqb_spec y v) ; nodec.
+  subst. constructor. reflexivity.
+Defined.
+
+Lemma eq_prod_refl :
+  forall A B (eqA : A -> A -> bool) (eqB : B -> B -> bool),
+    (forall a, eqA a a) ->
+    (forall b, eqB b b) ->
+    forall p, eq_prod eqA eqB p p.
+Proof.
+  intros A B eqA eqB eqA_refl eqB_refl [a b].
+  simpl. rewrite eqA_refl. apply eqB_refl.
+Qed.
+
